replaced Idx by nat

Execution_resources.v
@@ -3,6 +3,9 @@ From Views Require Import utils.
 Require Import PeanoNat.
 From Views Require Import BoundedInt.
 
+
+
+
 (* Inductive execlevel: Type :=
   | Blocks
   | Warps
@@ -20,22 +23,35 @@ Inductive execexpr: Type :=
 Inductive exec_distrib: Type :=
   | Distrib (ed: exec_distrib) (distribs: list (execlevel * nat)). *)
 
-Inductive Thread_t : Type :=
-  | t (id : nat)
-.
 
 
 Definition shape : Type := nat * nat * nat.
+Notation "XYZ< x y z >" := (x,y,z).
+Notation "XY< x y >" := (x,y,1).
+Notation "XZ< x z >" := (x,1,z).
+Notation "YZ< y z >" := (1,y,z).
+Notation "X< x >" := (x,1,1).
+Notation "Y< y >" := (1,y,1).
+Notation "Z< z >" := (1,1,z).
+
+Definition XYZ (x y z : nat) := (x,y,z).
+Definition XY (x y : nat) := (x,y,1).
+Definition XZ (x z : nat) := (x,1,z).
+Definition YZ (y z : nat) := (1,y,z).
+Definition X (x : nat) := (x,1,1).
+Definition Y (y : nat) := (1,y,1).
+Definition Z (z : nat) := (1,1,z).
 
 Definition Matrix (T : Type) (shp : shape) : Type :=
-  match shp with | (x,y,z) => Idx x -> Idx y -> Idx z -> T
+  match shp with | (x,y,z) => nat -> nat -> nat -> T
 end.
 
 Definition Vector (T : Type) (n : nat) : Type :=
-  Idx n -> T
+  nat -> T
 .
 
-Definition Warp_t : Type := Vector Thread_t 32.
+Definition Thread_t : Type := nat.
+Definition Warp_t (n : nat) : Type := Vector Thread_t n.
 Definition Block_t (shp : shape) : Type :=
       match shp with | (x,y,z) => Matrix Thread_t (x, y, z) end.
 Definition Grid_t (shp : shape) (shp' : shape) : Type :=
@@ -43,7 +59,7 @@ Definition Grid_t (shp : shape) (shp' : shape) : Type :=
 
 Inductive execution_resource : Type :=
   | thread (t : Thread_t)
-  | warp (w : Warp_t)
+  | warp (n : nat) (w : Warp_t n)
   | block (shp : shape) (b : Block_t shp)
   | grid (shp : shape) (shp' : shape) (g : Grid_t shp shp')
   | Collection (n : nat) (content : Vector execution_resource n)
@@ -53,50 +69,49 @@ Inductive execution_resource : Type :=
 
 Definition build_block (shp : shape) (offset : nat) : Block_t shp :=
   match shp with
-  | (x,y,z) => fun i j k => (t (offset + to_nat i + x*(to_nat j) + x*y*(to_nat k)))
+  | (x,y,z) => fun i j k => (offset + i + x*j + x*y*k)
 end.
 
 Definition build_grid (shp : shape) (shp' : shape) : Grid_t shp shp' :=
   match shp with
-  | (x,y,z) => fun i j k => (build_block shp' (to_nat i + x*(to_nat j) + x*y*(to_nat k)))
+  | (x,y,z) => fun i j k => (build_block shp' (i + x* j + x*y*k))
 end.
 
-Definition build_warp : Warp_t :=
-  fun i => (t (to_nat i))
+Definition build_warp (n : nat) : Warp_t n :=
+  fun i => i
 .
 
-Definition Thread (id : nat) := thread (t id).
-Definition Warp := warp build_warp.
+Definition Thread (id : nat) := thread id.
+Definition Warp (sz : nat) := warp sz (build_warp sz).
 Definition Block (shp : shape) := block shp (build_block shp 0).
 Definition Grid (shp : shape) (shp' : shape) := grid shp shp' (build_grid shp shp').
 
-Inductive dimension : Type :=
+Inductive dimension :=
   | _x | _y | _z
 .
-
 
 Fixpoint for_all (e : execution_resource) (d : dimension) : execution_resource :=
   match e,d with
   | Collection n v,_ => Collection n (fun x => for_all (v x) d)
-  | grid (x,1,1) shp' g, _x => Collection x (fun i => block shp' (g i zero zero))
-  | grid (1,y,1) shp' g, _y => Collection y (fun j => block shp' (g zero j zero))
-  | grid (1,1,z) shp' g, _z => Collection z (fun k => block shp' (g zero zero k))
+  | grid (x,1,1) shp' g, _x => Collection x (fun i => block shp' (g i 0 0))
+  | grid (1,y,1) shp' g, _y => Collection y (fun j => block shp' (g 0 j 0))
+  | grid (1,1,z) shp' g, _z => Collection z (fun k => block shp' (g 0 0 k))
   | grid (1,_,_) _ _, _x => Error
   | grid (_,1,_) _ _, _y => Error
   | grid (_,_,1) _ _, _z => Error
   | grid (x,y,z) shp' g, _x => Collection x (fun i => grid (1,y,z) shp' (fun _ j k => g i j k))
   | grid (x,y,z) shp' g, _y => Collection y (fun j => grid (x,1,z) shp' (fun i _ k => g i j k))
   | grid (x,y,z) shp' g, _z => Collection z (fun k => grid (x,y,1) shp' (fun i j _ => g i j k))
-  | block (x,1,1) b, _x => Collection x (fun i => thread (b i zero zero))
-  | block (1,y,1) b, _y => Collection y (fun j => thread (b zero j zero))
-  | block (1,1,z) b, _z => Collection z (fun k => thread (b zero zero k))
+  | block (x,1,1) b, _x => Collection x (fun i => thread (b i 0 0))
+  | block (1,y,1) b, _y => Collection y (fun j => thread (b 0 j 0))
+  | block (1,1,z) b, _z => Collection z (fun k => thread (b 0 0 k))
   | block (1,_,_) _, _x => Error
   | block (_,1,_) _, _y => Error
   | block (_,_,1) _, _z => Error
   | block (x,y,z) b, _x => Collection x (fun i => block (1,y,z) (fun _ j k => b i j k))
   | block (x,y,z) b, _y => Collection y (fun j => block (x,1,z) (fun i _ k => b i j k))
   | block (x,y,z) b, _z => Collection z (fun k => block (x,y,1) (fun i j _ => b i j k))
-  | warp w, _x => Collection 32 (fun i => thread (w i))
+  | warp sz w, _x => Collection sz (fun i => thread (w i))
   | _,_ => Error
 end.
 
@@ -107,49 +122,91 @@ Inductive Nested_List (T : Type) : Type :=
 
 Fixpoint to_list (e : execution_resource) : Nested_List execution_resource :=
   match e with
-  | Collection n v => Nest _ (rev (buildList (fun i => to_list (v i))))
+  | Collection n v => Nest _ (rev (buildList n (fun i => to_list (v i))))
   | _ => Elt _ e
 end.
 
 Notation "[ l ]" := (Nest _ l).
-Notation "# x" := (Elt _ x) (at level 20).
+Notation "@ x" := (Elt _ x) (at level 20).
 
-Definition err_b (shp : shape) : Block_t shp := match shp with | (x,y,z) => fun i j k => t 0 end.
+Fixpoint leb (x : nat) (y : nat) : bool :=
+  match x,y with
+  | 0,_ => true
+  | _,0 => false
+  | S x, S y => (leb x y)
+end.
+
+Notation "x <=? y" := (leb x y).
+
+Definition assert (cond : bool) (success : execution_resource) : execution_resource :=
+  if cond then success else Error.
 
 Fixpoint select (e : execution_resource) (l : nat) (r : nat) (d : dimension) : execution_resource :=
   match e,d with
   | Collection n v,_ => Collection n (fun x => select (v x) l r d)
-  | grid (_,1,1) shp' g, _x => Collection (r-l) (fun i => block shp' ((shift (fun i j => err_b shp') g) i zero zero))
-  | grid (1,_,1) shp' g, _y => Collection (r-l) (fun j => block shp' ((shift (fun j => err_b shp') (g zero)) j zero))
-  | grid (1,1,_) shp' g, _z => Collection (r-l) (fun k => block shp' ((shift (err_b shp') (g zero zero)) k))
+  | grid (x,1,1) shp' g, _x => assert (r <=? x) (Collection (r-l) (fun i => block shp' (g (i+l) 0 0)))
+  | grid (1,y,1) shp' g, _y => assert (r <=? y) (Collection (r-l) (fun j => block shp' (g 0 (j+l) 0)))
+  | grid (1,1,z) shp' g, _z => assert (r <=? z) (Collection (r-l) (fun k => block shp' (g 0 0 (k+l))))
   | grid (1,_,_) _ _, _x => Error
   | grid (_,1,_) _ _, _y => Error
   | grid (_,_,1) _ _, _z => Error
-  | grid (_,y,z) shp' g, _x => Collection (r-l) (fun i => grid (1,y,z) shp' (fun _ j k => (shift (fun i j => err_b shp') g) i j k))
-  | grid (x,_,z) shp' g, _y => Collection (r-l) (fun j => grid (x,1,z) shp' (fun i _ k => (shift (fun j => err_b shp') (g i)) j k))
-  | grid (x,y,_) shp' g, _z => Collection (r-l) (fun k => grid (x,y,1) shp' (fun i j _ => (shift (err_b shp') (g i j)) k))
-  | block (_,1,1) b, _x => Collection (r-l) (fun i => thread ((shift (fun i j => t 0) b) i zero zero))
-  | block (1,_,1) b, _y => Collection (r-l) (fun j => thread ((shift (fun j => t 0) (b zero)) j zero))
-  | block (1,1,_) b, _z => Collection (r-l) (fun k => thread ((shift (t 0) (b zero zero)) k))
+  | grid (x,y,z) shp' g, _x => assert (r <=? x) (Collection (r-l) (fun i => grid (1,y,z) shp' (fun _ j k => g (i+l) j k)))
+  | grid (x,y,z) shp' g, _y => assert (r <=? y) (Collection (r-l) (fun j => grid (x,1,z) shp' (fun i _ k => g i (j+l) k)))
+  | grid (x,y,z) shp' g, _z => assert (r <=? z) (Collection (r-l) (fun k => grid (x,y,1) shp' (fun i j _ => g i j (k+l))))
+  | block (x,1,1) b, _x => assert (r <=? x) (Collection (r-l) (fun i => thread (b (i+l) 0 0)))
+  | block (1,y,1) b, _y => assert (r <=? y) (Collection (r-l) (fun j => thread (b 0 (j+l) 0)))
+  | block (1,1,z) b, _z => assert (r <=? z) (Collection (r-l) (fun k => thread (b 0 0 (k+l))))
   | block (1,_,_) _, _x => Error
   | block (_,1,_) _, _y => Error
   | block (_,_,1) _, _z => Error
-  | block (_,y,z) b, _x => Collection (r-l) (fun i => block (1,y,z) (fun _ j k => (shift (fun i j => t 0) b) i j k))
-  | block (x,_,z) b, _y => Collection (r-l) (fun j => block (x,1,z) (fun i _ k => (shift (fun j => t 0) (b i)) j k))
-  | block (x,y,_) b, _z => Collection (r-l) (fun k => block (x,y,1) (fun i j _ => (shift (t 0) (b i j)) k))
-  | warp w, _x => Collection 32 (fun i => thread (w i))
+  | block (x,y,z) b, _x => assert (r <=? x) (Collection (r-l) (fun i => block (1,y,z) (fun _ j k => b (i+l) j k)))
+  | block (x,y,z) b, _y => assert (r <=? y) (Collection (r-l) (fun j => block (x,1,z) (fun i _ k => b i (j+l) k)))
+  | block (x,y,z) b, _z => assert (r <=? z) (Collection (r-l) (fun k => block (x,y,1) (fun i j _ => b i j (k+l))))
+  | warp sz w, _x => Collection sz (fun i => thread (w i))
   | _,_ => Error
 end.
 
-Example test :
-  to_list (select (Block (1,1,32)) 2 5 _z) = [[]].
+Example test1 :
+  to_list (Block (XZ 2 4)) =
+  @ block (XZ 2 4) (fun i j k : nat => i + 2*j + 2*k).
 Proof.
-  simpl; unfold crop; unfold shift; simpl; unfold crop_left;
-  unfold take_left; unfold rtake_left;
-  unfold take_right; unfold rtake_right;
-  simpl; unfold expand;
-  unfold reverse; unfold expand_left; simpl; unfold crop; unfold crop_left;
   simpl.
+  reflexivity.
+Qed.
+
+Example test2 :
+  to_list (select (Block (XZ 2 4)) 1 3 _z) =
+  [@ block (X 2) (fun i j _ : nat => i + 2*j + 2) :: @ block (X 2) (fun i j _ : nat => i + 2*j + 4) :: []].
+Proof.
+  simpl.
+  reflexivity.
+Qed.
+
+Example test3 :
+  to_list (for_all (select (Block (XZ 2 4)) 1 3 _z) _x) =
+  [[@ thread 2 :: @ thread 3 :: []] :: [@ thread 4 :: @ thread 5 :: []] :: []].
+Proof.
+  simpl.
+  reflexivity.
+Qed.
+
+
+
+
+
+
+
+
+
+
+
+
+
+
+
+
+
+
 
 
 
